add more timeless support

SpanningTree/Mon.thy
@@ -22,32 +22,52 @@ lemma n_incl_fragm_l: "n_incl n (fragm {l}) a = (case a of Auth (b,c) \<Rightarr
   by (auto split: auth.splits)
 
 text \<open> Marking Definitions \<close>
-definition is_marked ::"loc \<Rightarrow> iprop" where "is_marked l = Own\<^sub>m(fragm {l})"
+definition is_marked ::"loc \<Rightarrow> iprop" where "is_marked l = Own\<^sub>m(fragm {|l|})"
 
-lemma is_marked_split: "Own\<^sub>m(fragm {l}) = Own\<^sub>m(fragm {l} \<cdot> fragm {l})"
-  by (auto simp: auth_frag_op[symmetric] op_set_def)
+lemma is_marked_split: "Own\<^sub>m(fragm {|l|}) = Own\<^sub>m(fragm {|l|} \<cdot> fragm {|l|})"
+  by (auto simp: auth_frag_op[symmetric] op_fset_def)
 
 lemma dup_marked: "is_marked l \<stileturn>\<turnstile> is_marked l \<^emph> is_marked l"
 proof -
-from own_op have "Own (constr_markings marking_name (fragm {l}) \<cdot> constr_markings marking_name (fragm {l})) 
-    \<stileturn>\<turnstile> (Own\<^sub>m(fragm {l})) \<^emph> Own\<^sub>m(fragm {l})" 
+from own_op have "Own (constr_markings marking_name (fragm {|l|}) \<cdot> 
+  constr_markings marking_name (fragm {|l|})) \<stileturn>\<turnstile> (Own\<^sub>m(fragm {|l|})) \<^emph> Own\<^sub>m(fragm {|l|})" 
   by auto
-then have "Own(constr_markings marking_name (fragm {l}\<cdot>fragm {l})) \<stileturn>\<turnstile> Own\<^sub>m(fragm {l}) \<^emph> Own\<^sub>m(fragm {l})" 
+then have "Own(constr_markings marking_name (fragm {|l|}\<cdot>fragm {|l|})) \<stileturn>\<turnstile> Own\<^sub>m(fragm {|l|}) \<^emph> Own\<^sub>m(fragm {|l|})" 
   by (auto simp add: op_prod_def \<epsilon>_left_id constr_markings_def)
 then show ?thesis unfolding is_marked_split[symmetric] by (simp add: is_marked_def)
 qed
 
-type_synonym gmon = "loc\<rightharpoonup>(chl ex)"
+type_synonym gmon = "(loc,(chl ex)) fmap"
 
 fun excl_chlC_chl :: "chl ex \<Rightarrow> chl option" where
   "excl_chlC_chl (Ex w) = Some w"
 | "excl_chlC_chl ex.Inv = None"
 
-definition gmon_graph :: "gmon \<Rightarrow> loc graph" where 
-  "gmon_graph g = (\<lambda>l. Option.bind l excl_chlC_chl) \<circ> g"
-lemma gmon_graph_dom: "valid g \<Longrightarrow> (dom (gmon_graph g) = dom g)"
-  by (auto simp: gmon_graph_def valid_def valid_raw_fun_def valid_raw_option_def bind_eq_Some_conv 
-  Abs_sprop_inverse valid_raw_ex_def split: ex.splits option.splits) (metis excl_chlC_chl.elims surj_pair)
+context includes fmap.lifting begin
+lift_definition gmon_graph :: "gmon \<Rightarrow> loc graph_map" is
+  "\<lambda>g. (\<lambda>l. Option.bind l excl_chlC_chl) \<circ> g" .
+end
+thm gmon_graph.rep_eq
+lemma gmon_graph_dom: "valid g \<Longrightarrow> (dom (gmon_graph g) = fmdom' g)"
+proof -
+  assume assm: "valid g"
+  then have "\<forall>i. valid (fmlookup g i)" 
+    by (auto simp: valid_def valid_raw_fmap_def valid_raw_fun.rep_eq)
+  then have "\<forall>j\<in>fmran' g. valid j" 
+    by (auto simp: fmran'_def valid_def valid_raw_option_def split: option.splits)
+  then have "\<forall>j\<in>fmran' g. j \<noteq> ex.Inv" by (auto simp: valid_def valid_raw_ex_def)
+  then have "\<forall>j\<in>fmran' g. \<exists>j'. j= Ex j' \<and> excl_chlC_chl j = Some j'" by (meson excl_chlC_chl.elims)
+  then have "\<forall>i\<in>fmdom' g. \<exists>j'. fmlookup g i = Some (Ex j') \<and> excl_chlC_chl (the (fmlookup g i)) = Some j'"
+    apply auto by (metis fmlookup_dom'_iff fmran'I option.sel)
+  then have "\<forall>i\<in>fmdom' g. \<exists>j'. ((\<lambda>l. Option.bind l excl_chlC_chl) \<circ> fmlookup g) i = Some j'"
+    by auto
+  then have rtol: "fmdom' g \<subseteq> dom (gmon_graph g)" by (auto simp: gmon_graph.rep_eq)
+  have "\<nexists>j'. Option.bind None excl_chlC_chl = Some j'" by auto
+  then have "\<forall>i\<in> -fmdom' g. \<nexists>j'. ((\<lambda>l. Option.bind l excl_chlC_chl) \<circ> fmlookup g) i = Some j'"
+    by auto
+  then have "dom (gmon_graph g) \<subseteq> fmdom' g" apply (auto simp: gmon_graph.rep_eq) by blast  
+  with rtol show ?thesis by auto
+qed
 
 fun child_to_val :: "loc option \<Rightarrow> val" where
   "child_to_val None = NoneV"
@@ -56,28 +76,41 @@ fun child_to_val :: "loc option \<Rightarrow> val" where
 definition children_to_val :: "chl \<Rightarrow> val" where
   "children_to_val chs = PairV (child_to_val (fst chs)) (child_to_val (snd chs))"
 
-type_synonym marked_graph = "loc\<rightharpoonup>(bool\<times>chl)"
+type_synonym marked_graph = "(loc,(bool\<times>chl)) fmap"
 
-definition of_graph_elem :: "gmon \<Rightarrow> loc \<Rightarrow> chl \<Rightarrow> (bool\<times>chl) option" where
-  "of_graph_elem g l v = (case gmon_graph g l of Some w \<Rightarrow> Some (True,w) | None \<Rightarrow> Some (False, v))"
+definition of_graph_elem :: "gmon \<Rightarrow> loc \<Rightarrow> chl \<Rightarrow> (bool\<times>chl)" where
+  "of_graph_elem g l v = (case gmon_graph g l of Some w \<Rightarrow> (True,w) | None \<Rightarrow> (False, v))"
 
 definition of_graph :: "loc graph \<Rightarrow> gmon \<Rightarrow> marked_graph" where
-  "of_graph g G l = Option.bind (g l) (\<lambda>chl. of_graph_elem G l chl)"
+  "of_graph g G = fmmap_keys (\<lambda>l chl. of_graph_elem G l chl) g"
 
 definition own_graphUR :: "frac \<Rightarrow> gmon \<Rightarrow> iprop" where
   "own_graphUR q G = Own\<^sub>g(fragm (Some (G,q)))"
 
 definition heap_owns :: "marked_graph \<Rightarrow> (loc\<rightharpoonup>loc) \<Rightarrow> iprop" where
   "heap_owns M markings = 
-  sep_map_set (\<lambda>(l,(b,cl)). (\<exists>\<^sub>u m. ((\<upharpoonleft>(markings l = Some m))
+  sep_map_fset (\<lambda>(l,(b,cl)). (\<exists>\<^sub>u m. ((\<upharpoonleft>(markings l = Some m))
     \<^emph> (l\<mapsto>\<^sub>u#[(m, children_to_val cl)])
     \<^emph> (m\<mapsto>\<^sub>u#[b]))))
-  {(l,node) | l node. M l = Some node}"
+  (fset_of_fmap M)"
 
 definition graph_inv :: "loc graph \<Rightarrow> (loc\<rightharpoonup>loc) \<Rightarrow> iprop" where
   "graph_inv g markings \<equiv> \<exists>\<^sub>u (G::gmon). ((Own\<^sub>g(full (Some (G, 1))))
-    \<^emph> (Own\<^sub>m(full (dom G))) \<^emph> (heap_owns (of_graph g G) markings) 
-    \<^emph> (\<upharpoonleft>(strict_subgraph g (gmon_graph G))))"
+    \<^emph> (Own\<^sub>m(full (fmdom G))) \<^emph> (heap_owns (of_graph g G) markings) 
+    \<^emph> (\<upharpoonleft>(strict_subgraph' g (gmon_graph G))))"
+
+lemma own_graph_timeless [timeless_rule]:"timeless (Own\<^sub>g g)"
+  unfolding timeless_def except_zero_def constr_graph_def
+  by transfer (auto simp: singleton_map_n_incl d_equiv)
+
+lemma own_markings_timeless [timeless_rule]:"timeless (Own\<^sub>m m)"
+  unfolding timeless_def except_zero_def constr_markings_def
+  by transfer (auto simp: singleton_map_n_incl d_equiv)
+
+lemma graph_inv_timeless [timeless_rule]: "timeless (graph_inv g m)"
+  unfolding graph_inv_def heap_owns_def
+  apply timeless_solver
+  apply auto by timeless_solver
 
 definition graph_ctxt :: "gname \<Rightarrow> loc graph \<Rightarrow> (loc\<rightharpoonup>loc) \<Rightarrow> iprop" where 
   "graph_ctxt \<kappa> g Mrk \<equiv> cinv graphN \<kappa> (graph_inv g Mrk)"
@@ -85,6 +118,6 @@ definition graph_ctxt :: "gname \<Rightarrow> loc graph \<Rightarrow> (loc\<righ
 lemma graph_ctxt_persistent [pers_rule]: "persistent (graph_ctxt \<kappa> g Mrk)"
   unfolding graph_ctxt_def by (rule cinv_persistent)
 
-definition gmon_map :: "loc \<Rightarrow> chl \<Rightarrow> gmon" where "gmon_map l v = [l\<mapsto>Ex v]"
+definition gmon_map :: "loc \<Rightarrow> chl \<Rightarrow> gmon" where "gmon_map l v = fmupd l (Ex v) fmempty"
 notation gmon_map (infix "[\<mapsto>\<^sub>g]" 60)
 end    
