SpanningTree/SpanningTreeCameras.thy
@@ -8,10 +8,10 @@ begin
 type_synonym chl = "loc option\<times>loc option"
 
 (* The graph camera, a unital camera. *)
-type_synonym graphUR = "((loc\<rightharpoonup>(chl ex))\<times>frac) option"
+type_synonym graphUR = "(((loc,(chl ex))fmap)\<times>frac) option"
 
 (* A camera for duplicatable markings *)
-type_synonym markingUR = "loc set"
+type_synonym markingUR = "loc fset"
 
 type_synonym spanningG = "(graphUR auth \<times> markingUR auth)"
 end
