IrisCore/Automation.thy
@@ -7,11 +7,17 @@ method itac = tactic all_tac
 method iIntro = 
   (match conclusion in "upred_holds _" \<Rightarrow> \<open>rule upred_wand_holdsI\<close>)?,((rule upred_wandI)+)?
   
-method entails_substL uses rule = 
-  (match rule in "_ = _" \<Rightarrow> \<open>rule upred_entails_trans[OF upred_entails_eq[OF rule]]\<close>
-   \<bar> "_ \<turnstile> _" \<Rightarrow> \<open>rule upred_entails_trans[OF rule]\<close>)
-| rule upred_entails_substE[OF rule, unfolded upred_sep_assoc_eq]
-| rule upred_entails_substE'[OF rule, unfolded upred_conj_assoc]
+method entails_substL uses rule rule_eq = 
+  (match rule_eq in "_ = _" \<Rightarrow> \<open>rule upred_entails_trans[OF upred_entails_eq[OF rule_eq]]\<close>)
+| (match rule in "_" \<Rightarrow> \<open>rule upred_entails_substE[OF rule, unfolded upred_sep_assoc_eq]\<close>)
+| (match rule in "_" \<Rightarrow> \<open>rule upred_entails_trans[OF rule]\<close>)
+| (match rule in "_" \<Rightarrow> \<open>rule upred_entails_substE'[OF rule, unfolded upred_conj_assoc]\<close>)
+
+method dupl_pers = (entails_substL rule: upred_entail_eqR[OF persistent_dupl], (pers_solver; fail))?
+
+method subst_pers_keep uses rule =
+  (entails_substL rule: persistent_keep[OF _ rule], pers_solver)
+| entails_substL rule: rule
 
 method move_sepL for pat :: "'a::ucamera upred_f" =
   match conclusion in \<open>hyps \<turnstile> goal\<close> for hyps goal \<Rightarrow>
@@ -19,24 +25,41 @@ method move_sepL for pat :: "'a::ucamera upred_f" =
       \<bar> "_\<^emph>pat" \<Rightarrow> itac
       \<bar> "pat\<^emph>_" \<Rightarrow> \<open>subst upred_sep_comm\<close>
       \<bar> "_\<^emph>pat\<^emph>_" \<Rightarrow> \<open>entails_substL rule: upred_sep_comm2R\<close>
-      \<bar> "pat\<^emph>_\<^emph>_" \<Rightarrow> \<open>entails_substL rule: upred_sep_comm2L; move_sepL pat\<close>
+      \<bar> "pat\<^emph>_\<^emph>_" \<Rightarrow> \<open>entails_substL rule_eq: upred_sep_comm2L; move_sepL pat\<close>
       \<bar> "_\<^emph>pat\<^emph>_\<^emph>_" \<Rightarrow> \<open>entails_substL rule: upred_sep_comm3M; move_sepL pat\<close>
       \<bar> "pat\<^emph>_\<^emph>_\<^emph>_" \<Rightarrow> \<open>entails_substL rule: upred_sep_comm3L; move_sepL pat\<close>
       \<bar> "_\<^emph>pat\<^emph>_\<^emph>_\<^emph>_" \<Rightarrow> \<open>entails_substL rule: upred_sep_comm4_2; move_sepL pat\<close>
       \<bar> "pat\<^emph>_\<^emph>_\<^emph>_\<^emph>_" \<Rightarrow> \<open>entails_substL rule: upred_sep_comm4_1; move_sepL pat\<close>
+      \<bar> "_\<^emph>pat\<^emph>_\<^emph>_\<^emph>_\<^emph>_" \<Rightarrow> \<open>entails_substL rule: upred_sep_comm5_2; move_sepL pat\<close>
+      \<bar> "pat\<^emph>_\<^emph>_\<^emph>_\<^emph>_\<^emph>_" \<Rightarrow> \<open>entails_substL rule: upred_sep_comm5_1; move_sepL pat\<close>
+      \<bar> "_\<^emph>pat\<^emph>_\<^emph>_\<^emph>_\<^emph>_\<^emph>_" \<Rightarrow> \<open>entails_substL rule: upred_sep_comm6_2; move_sepL pat\<close>
+      \<bar> "pat\<^emph>_\<^emph>_\<^emph>_\<^emph>_\<^emph>_\<^emph>_" \<Rightarrow> \<open>entails_substL rule: upred_sep_comm6_1; move_sepL pat\<close>
     \<close>
 
-method apply_wand = (move_sepL "?P-\<^emph>?Q");
-  match conclusion in \<open>hyps \<turnstile> goal\<close> for hyps goal \<Rightarrow>
-    \<open> match (hyps) in "P\<^emph>(Q-\<^emph>R)" for P Q R \<Rightarrow> \<open>(move_sepL Q; 
-      entails_substL rule: upred_sep_comm2R; entails_substL rule: upred_wand_apply)\<close> \<close>
+method find_pat_sep for pat trm :: "'a::ucamera upred_f" = 
+  match (trm) in "pat" \<Rightarrow> itac
+  \<bar> "_\<^emph>pat" \<Rightarrow> itac
+  \<bar> "pat\<^emph>_" \<Rightarrow> itac
+  \<bar> "rest\<^emph>_" for rest :: "'a upred_f" \<Rightarrow> \<open>find_pat_sep pat rest\<close>   
 
-method iFrame_simp = match conclusion in \<open>hyps \<turnstile> goal\<close> for hyps goal \<Rightarrow>
-    \<open> match (goal) in "_\<^emph>P" for P \<Rightarrow> \<open>move_sepL P; rule upred_frame\<close> 
-      \<bar> _ \<Rightarrow> \<open>rule upred_entails_refl | rule upred_weakeningL | rule upred_weakeningR\<close>\<close>
+method find_applicable_wand for whole trm :: "'a::ucamera upred_f" =
+  match (trm) in "P-\<^emph>Q" for P Q :: "'a upred_f" \<Rightarrow>
+    \<open>find_pat_sep P whole; move_sepL P; dupl_pers; move_sepL "P-\<^emph>Q"\<close>
+  \<bar> "_\<^emph>(P-\<^emph>Q)" for P Q :: "'a upred_f" \<Rightarrow>
+    \<open>find_pat_sep P whole; move_sepL P; dupl_pers; move_sepL "P-\<^emph>Q"\<close>
+  \<bar> "rest\<^emph>_" for rest :: "'a upred_f" \<Rightarrow> \<open>find_applicable_wand whole rest\<close>
+
+method iApply_wand =
+  match conclusion in \<open>hyps \<turnstile> goal\<close> for hyps goal \<Rightarrow>
+    \<open>find_applicable_wand hyps hyps; subst_pers_keep rule: upred_wand_apply\<close>
+
+method iFrame_single = match conclusion in \<open>hyps \<turnstile> goal\<close> for hyps goal :: "'a::ucamera upred_f" \<Rightarrow>
+    \<open> match (goal) in "_\<^emph>P" for P \<Rightarrow> \<open>move_sepL P; dupl_pers; rule upred_frame\<close> 
+      \<bar> P for P :: "'a upred_f" \<Rightarrow> 
+      \<open>move_sepL P; rule upred_entails_refl | rule upred_weakeningL | rule upred_weakeningR\<close> \<close>
     
-lemma test_lemma: "S \<^emph> P \<^emph> Q \<^emph> (P-\<^emph>R) \<^emph> (\<triangleright>R) -\<^emph> R \<^emph> (\<triangleright>R) \<^emph> Q"
+lemma test_lemma: "S \<^emph> (\<box>P) \<^emph> Q \<^emph> ((\<box>P)-\<^emph>\<box>R) \<^emph> (\<triangleright>R) -\<^emph> (\<box>R) \<^emph> (\<triangleright>R) \<^emph> Q"
 apply iIntro
-apply apply_wand
-by iFrame_simp+
+apply iApply_wand
+by iFrame_single+
 end
