SpanningTree/Graph.thy
@@ -1,5 +1,5 @@
 theory Graph
-imports Main
+imports Main "HOL-Library.Finite_Map"
 begin
 
 section \<open> Spanning Tree example\<close>
@@ -8,13 +8,19 @@ text \<open> A simple example application of the Iris base logic;
 
 subsection \<open> Graph definition \<close>
 
-type_synonym 'a graph = "'a \<rightharpoonup> ('a option\<times>'a option)"
+type_synonym 'a graph = "('a,('a option\<times>'a option)) fmap"
+type_synonym 'a graph_map = "'a\<rightharpoonup>('a option\<times>'a option)"
 
 definition get_left :: "'a graph \<Rightarrow> 'a \<Rightarrow> 'a option" where
-  "get_left g x = Option.bind (g x) fst"
+  "get_left g x = Option.bind (fmlookup g x) fst"
 definition get_right :: "'a graph \<Rightarrow> 'a \<Rightarrow> 'a option" where
-  "get_right g x = Option.bind (g x) snd"
+  "get_right g x = Option.bind (fmlookup g x) snd"
 
+definition get_left' :: "'a graph_map \<Rightarrow> 'a \<Rightarrow> 'a option" where
+  "get_left' g x = Option.bind (g x) fst"
+definition get_right' :: "'a graph_map \<Rightarrow> 'a \<Rightarrow> 'a option" where
+  "get_right' g x = Option.bind (g x) snd"
+  
 fun strict_sub_child :: "'a option \<Rightarrow> 'a option \<Rightarrow> bool" where
   "strict_sub_child (Some c) (Some c') = (c=c')"
 | "strict_sub_child (Some _) None = True"
@@ -29,24 +35,28 @@ definition strict_subgraph :: "'a graph \<Rightarrow> 'a graph \<Rightarrow> boo
   "strict_subgraph g1 g2 \<equiv> 
     \<forall>x. strict_sub_children (get_left g1 x, get_right g1 x) (get_left g2 x, get_right g2 x)"
 
+definition strict_subgraph' :: "'a graph \<Rightarrow> 'a graph_map \<Rightarrow> bool" where
+  "strict_subgraph' g1 g2 \<equiv> 
+    \<forall>x. strict_sub_children (get_left g1 x, get_right g1 x) (get_left' g2 x, get_right' g2 x)"
+    
 (* Path defined by whether a step went left (True) or right (False). Empty path stays at the node. *)
 type_synonym path = "bool list"
 
 inductive valid_path :: "'a graph \<Rightarrow> 'a \<Rightarrow> 'a \<Rightarrow> path \<Rightarrow> bool" where
-  valid_pathE: "\<lbrakk>x\<in>dom g; x=y\<rbrakk> \<Longrightarrow> valid_path g x y []"
+  valid_pathE: "\<lbrakk>x\<in>fmdom' g; x=y\<rbrakk> \<Longrightarrow> valid_path g x y []"
 | valid_pathL: "\<lbrakk>get_left g x = Some xl; valid_path g xl y p\<rbrakk> \<Longrightarrow> valid_path g x y (True#p)"
 | valid_pathR: "\<lbrakk>get_right g x = Some xr; valid_path g xr y p\<rbrakk> \<Longrightarrow> valid_path g x y (False#p)"
 
 definition connected :: "'a graph \<Rightarrow> 'a \<Rightarrow> bool" where
-  "connected g x \<equiv> \<forall>z\<in>dom g. \<exists>p. valid_path g x z p"
+  "connected g x \<equiv> \<forall>z\<in> fmdom' g. \<exists>p. valid_path g x z p"
 
 definition front :: "'a graph \<Rightarrow> 'a set \<Rightarrow> 'a set \<Rightarrow> bool" where
-  "front g t1 t2 \<equiv> t1\<subseteq>dom g \<and> (\<forall>x\<in>t1. \<forall>v. ((get_left g x = Some v) \<or> (get_right g x = Some v)) \<longrightarrow> v\<in>t2)"
+  "front g t1 t2 \<equiv> t1\<subseteq>fmdom' g \<and> (\<forall>x\<in>t1. \<forall>v. ((get_left g x = Some v) \<or> (get_right g x = Some v)) \<longrightarrow> v\<in>t2)"
 
-definition maximal :: "'a graph \<Rightarrow> bool" where "maximal g \<equiv> front g (dom g) (dom g)"
+definition maximal :: "'a graph \<Rightarrow> bool" where "maximal g \<equiv> front g (fmdom' g) (fmdom' g)"
 
 definition tree :: "'a graph \<Rightarrow> 'a \<Rightarrow> bool" where
-  "tree g x \<equiv> \<forall>z\<in>dom g. (\<exists>p. valid_path g x z p \<and> (\<forall>p'. valid_path g x z p' \<longrightarrow> (p=p')))"
+  "tree g x \<equiv> \<forall>z\<in>fmdom' g. (\<exists>p. valid_path g x z p \<and> (\<forall>p'. valid_path g x z p' \<longrightarrow> (p=p')))"
 
 (* Lemmas omitted for now, will only add as axioms when needed. *)
 end
